Weidenbach_Book/IsaSAT/IsaSAT_Rephase.thy
@@ -1,8 +1,28 @@
 theory IsaSAT_Rephase
-  imports IsaSAT_Setup IsaSAT_Show
+  imports IsaSAT_Literals Watched_Literals_VMTF
 begin
 
-chapter \<open>Rephasing\<close>
+chapter \<open>Phase Saving\<close>
+
+section \<open>Rephasing\<close>
+
+type_synonym phase_save_heur = \<open>phase_saver \<times> nat \<times> phase_saver \<times> nat \<times> phase_saver \<times> 64 word \<times> 64 word \<times> 64 word\<close>
+
+definition phase_save_heur_rel :: \<open>nat multiset \<Rightarrow> phase_save_heur \<Rightarrow> bool\<close> where
+\<open>phase_save_heur_rel \<A> = (\<lambda>(\<phi>, target_assigned, target, best_assigned, best,
+    end_of_phase, curr_phase). phase_saving \<A> \<phi> \<and>
+  phase_saving \<A> target \<and> phase_saving \<A> best \<and> length \<phi> = length best \<and>
+  length target = length best)\<close>
+
+definition end_of_rephasing_phase :: \<open>phase_save_heur \<Rightarrow> 64 word\<close> where
+  \<open>end_of_rephasing_phase = (\<lambda>(\<phi>, target_assigned, target, best_assigned, best, end_of_phase, curr_phase,
+     length_phase). end_of_phase)\<close>
+
+
+definition phase_current_rephasing_phase :: \<open>phase_save_heur \<Rightarrow> 64 word\<close> where
+  \<open>phase_current_rephasing_phase =
+    (\<lambda>(\<phi>, target_assigned, target, best_assigned, best, end_of_phase, curr_phase, length_phase). curr_phase)\<close>
+
 
 text \<open>
   We implement the idea in CaDiCaL of rephasing:
@@ -220,37 +240,6 @@ proof -
     done
 qed
 
-definition rephase_heur :: \<open>64 word \<Rightarrow> restart_heuristics \<Rightarrow> restart_heuristics nres\<close> where
-  \<open>rephase_heur = (\<lambda>b (fast_ema, slow_ema, restart_info, wasted, \<phi>).
-    do {
-      \<phi> \<leftarrow> phase_rephase b \<phi>;
-      RETURN (fast_ema, slow_ema, restart_info, wasted, \<phi>)
-   })\<close>
-
-lemma rephase_heur_spec:
-  \<open>heuristic_rel \<A> heur \<Longrightarrow> rephase_heur b heur \<le>  \<Down>Id (SPEC(heuristic_rel \<A>))\<close>
-  unfolding rephase_heur_def
-  apply (refine_vcg phase_rephase_spec[THEN order_trans])
-  apply (auto simp: heuristic_rel_def)
-  done
-
-definition rephase_heur_st :: \<open>twl_st_wl_heur \<Rightarrow> twl_st_wl_heur nres\<close> where
-  \<open>rephase_heur_st = (\<lambda>(M', arena, D', j, W', vm, clvls, cach, lbd, outl, stats, heur,
-       vdom, avdom, lcount, opts, old_arena). do {
-      let b = current_restart_phase heur;
-      heur \<leftarrow> rephase_heur b heur;
-      let _ = isasat_print_progress (current_rephasing_phase heur) b stats lcount;
-      RETURN (M', arena, D', j, W', vm, clvls, cach, lbd, outl, stats, heur,
-       vdom, avdom, lcount, opts, old_arena)
-   })\<close>
-
-lemma rephase_heur_st_spec:
-  \<open>(S, S') \<in> twl_st_heur \<Longrightarrow> rephase_heur_st S \<le> SPEC(\<lambda>S. (S, S') \<in> twl_st_heur)\<close>
-  unfolding rephase_heur_st_def
-  apply (cases S')
-  apply (refine_vcg rephase_heur_spec[THEN order_trans, of \<open>all_atms_st S'\<close>])
-  apply (simp_all add:  twl_st_heur_def)
-  done
 
 definition phase_save_phase :: \<open>nat \<Rightarrow> phase_save_heur \<Rightarrow> phase_save_heur nres\<close> where
 \<open>phase_save_phase = (\<lambda>n (\<phi>, target_assigned, target, best_assigned, best, end_of_phase, curr_phase). do {
@@ -300,42 +289,5 @@ proof -
     apply (auto simp: phase_rephase_def)
     done
 qed
-
-definition save_rephase_heur :: \<open>nat \<Rightarrow> restart_heuristics \<Rightarrow> restart_heuristics nres\<close> where
-  \<open>save_rephase_heur = (\<lambda>n (fast_ema, slow_ema, restart_info, wasted, \<phi>).
-    do {
-      \<phi> \<leftarrow> phase_save_phase n \<phi>;
-      RETURN (fast_ema, slow_ema, restart_info, wasted, \<phi>)
-   })\<close>
-
-lemma save_phase_heur_spec:
-  \<open>heuristic_rel \<A> heur \<Longrightarrow> save_rephase_heur n heur \<le>  \<Down>Id (SPEC(heuristic_rel \<A>))\<close>
-  unfolding save_rephase_heur_def
-  apply (refine_vcg phase_save_phase_spec[THEN order_trans])
-  apply (auto simp: heuristic_rel_def)
-  done
-
-
-definition save_phase_st :: \<open>twl_st_wl_heur \<Rightarrow> twl_st_wl_heur nres\<close> where
-  \<open>save_phase_st = (\<lambda>(M', arena, D', j, W', vm, clvls, cach, lbd, outl, stats, heur,
-       vdom, avdom, lcount, opts, old_arena). do {
-      ASSERT(isa_length_trail_pre M');
-      let n = isa_length_trail M';
-      heur \<leftarrow> save_rephase_heur n heur;
-      RETURN (M', arena, D', j, W', vm, clvls, cach, lbd, outl, stats, heur,
-       vdom, avdom, lcount, opts, old_arena)
-   })\<close>
-
-lemma save_phase_st_spec:
-  \<open>(S, S') \<in> twl_st_heur \<Longrightarrow> save_phase_st S \<le> SPEC(\<lambda>S. (S, S') \<in> twl_st_heur)\<close>
-  unfolding save_phase_st_def
-  apply (cases S')
-  apply (refine_vcg save_phase_heur_spec[THEN order_trans, of \<open>all_atms_st S'\<close>])
-  apply (simp_all add:  twl_st_heur_def isa_length_trail_pre)
-  apply (rule isa_length_trail_pre)
-  apply blast
-  done
-
-
 
 end
