Weidenbach_Book/IsaSAT/IsaSAT_Rephase_LLVM.thy
@@ -1,6 +1,20 @@
 theory IsaSAT_Rephase_LLVM
-  imports IsaSAT_Rephase IsaSAT_Show_LLVM
+  imports IsaSAT_Rephase IsaSAT_Literals_LLVM
 begin
+
+type_synonym phase_saver_assn = \<open>1 word larray64\<close>
+abbreviation phase_saver_assn :: \<open>phase_saver \<Rightarrow> phase_saver_assn \<Rightarrow> assn\<close> where
+  \<open>phase_saver_assn \<equiv> larray64_assn bool1_assn\<close>
+
+type_synonym phase_saver'_assn = \<open>1 word ptr\<close>
+
+abbreviation phase_saver'_assn :: \<open>phase_saver \<Rightarrow> phase_saver'_assn \<Rightarrow> assn\<close> where
+  \<open>phase_saver'_assn \<equiv> array_assn bool1_assn\<close>
+
+
+abbreviation phase_heur_assn where
+  \<open>phase_heur_assn \<equiv> phase_saver_assn \<times>\<^sub>a sint64_nat_assn \<times>\<^sub>a phase_saver'_assn \<times>\<^sub>a sint64_nat_assn \<times>\<^sub>a
+     phase_saver'_assn \<times>\<^sub>a word64_assn \<times>\<^sub>a word64_assn \<times>\<^sub>a word64_assn\<close>
 
 sepref_def rephase_random_impl
   is \<open>uncurry rephase_random\<close>
@@ -54,64 +68,6 @@ sepref_def phase_save_phase_impl
   supply [[goals_limit=1]]
   unfolding phase_save_phase_def
   by sepref
-
-
-sepref_def save_phase_heur_impl
-  is \<open>uncurry save_rephase_heur\<close>
-  ::  \<open>sint64_nat_assn\<^sup>k *\<^sub>a heuristic_assn\<^sup>d \<rightarrow>\<^sub>a heuristic_assn\<close>
-  supply [[goals_limit=1]]
-  unfolding save_rephase_heur_def heuristic_assn_def
-  by sepref
-
-
-sepref_def save_phase_heur_st
-  is save_phase_st
-  ::  \<open>isasat_bounded_assn\<^sup>d \<rightarrow>\<^sub>a isasat_bounded_assn\<close>
-  supply [[goals_limit=1]]
-  unfolding save_phase_st_def isasat_bounded_assn_def
-  by sepref
-
-sepref_def phase_save_rephase_impl
-  is \<open>uncurry phase_rephase\<close>
-  :: \<open>word_assn\<^sup>k *\<^sub>a phase_heur_assn\<^sup>d \<rightarrow>\<^sub>a phase_heur_assn\<close>
-  unfolding phase_rephase_def copy_phase2_def[symmetric]
-  by sepref
-
-
-sepref_def rephase_heur_impl
-  is \<open>uncurry rephase_heur\<close>
-  :: \<open>word_assn\<^sup>k *\<^sub>a heuristic_assn\<^sup>d \<rightarrow>\<^sub>a heuristic_assn\<close>
-  unfolding rephase_heur_def heuristic_assn_def
-  by sepref
-
-lemma current_rephasing_phase_alt_def:
-  \<open>RETURN o current_rephasing_phase =
-    (\<lambda>(fast_ema, slow_ema, res_info, wasted,
-      (\<phi>, target_assigned, target, best_assigned, best, end_of_phase, curr_phase, length_phase)).
-      RETURN curr_phase)\<close>
-  unfolding current_rephasing_phase_def
-    phase_current_rephasing_phase_def
-  by (auto intro!: ext)
-
-sepref_def current_rephasing_phase
-  is \<open>RETURN o current_rephasing_phase\<close>
-  :: \<open>heuristic_assn\<^sup>k \<rightarrow>\<^sub>a word64_assn\<close>
-  unfolding current_rephasing_phase_alt_def heuristic_assn_def
-  by sepref
-
-sepref_register rephase_heur
-sepref_def rephase_heur_st_impl
-  is rephase_heur_st
-  ::  \<open>isasat_bounded_assn\<^sup>d \<rightarrow>\<^sub>a isasat_bounded_assn\<close>
-  unfolding rephase_heur_st_def isasat_bounded_assn_def
-  by sepref
-
-
-experiment
-begin
-export_llvm rephase_heur_st_impl
-  save_phase_heur_st
-end
 
 end
 
