Weidenbach_Book/IsaSAT/IsaSAT_EMA.thy
@@ -1,0 +1,55 @@
+theory IsaSAT_EMA
+  imports IsaSAT_Literals
+begin
+
+section \<open>Moving averages\<close>
+
+text \<open>We use (at least hopefully) the variant of EMA-14 implemented in Cadical, but with fixed-point
+calculation (\<^term>\<open>1 :: nat\<close> is \<^term>\<open>(1 :: nat) >> 32\<close>).
+
+Remark that the coefficient \<^term>\<open>\<beta>\<close> already should not take care of the fixed-point conversion of the glue.
+Otherwise, \<^term>\<open>value\<close> is wrongly updated.
+\<close>
+type_synonym ema = \<open>64 word \<times> 64 word \<times> 64 word \<times> 64 word \<times> 64 word\<close>
+
+definition ema_bitshifting where
+  \<open>ema_bitshifting = (1 << 32)\<close>
+
+
+definition (in -) ema_update :: \<open>nat \<Rightarrow> ema \<Rightarrow> ema\<close> where
+  \<open>ema_update = (\<lambda>lbd (value, \<alpha>, \<beta>, wait, period).
+     let lbd = (of_nat lbd) * ema_bitshifting in
+     let value = if lbd > value then value + (\<beta> * (lbd - value) >> 32) else value - (\<beta> * (value - lbd) >> 32) in
+     if \<beta> \<le> \<alpha> \<or> wait > 0 then (value, \<alpha>, \<beta>, wait - 1, period)
+     else
+       let wait = 2 * period + 1 in
+       let period = wait in
+       let \<beta> = \<beta> >> 1 in
+       let \<beta> = if \<beta> \<le> \<alpha> then \<alpha> else \<beta> in
+       (value, \<alpha>, \<beta>, wait, period))\<close>
+
+definition (in -) ema_init :: \<open>64 word \<Rightarrow> ema\<close> where
+  \<open>ema_init \<alpha> = (0, \<alpha>, ema_bitshifting, 0, 0)\<close>
+
+fun ema_reinit where
+  \<open>ema_reinit (value, \<alpha>, \<beta>, wait, period) = (value, \<alpha>, 1 << 32, 0, 0)\<close>
+
+fun ema_get_value :: \<open>ema \<Rightarrow> 64 word\<close> where
+  \<open>ema_get_value (v, _) = v\<close>
+
+fun ema_extract_value :: \<open>ema \<Rightarrow> 64 word\<close> where
+  \<open>ema_extract_value (v, _) = v >> 32\<close>
+
+
+text \<open>We use the default values for Cadical: \<^term>\<open>(3 / 10 ^2)\<close> and  \<^term>\<open>(1 / 10 ^ 5)\<close>  in our fixed-point
+  version.
+\<close>
+
+abbreviation ema_fast_init :: ema where
+  \<open>ema_fast_init \<equiv> ema_init (128849010)\<close>
+
+abbreviation ema_slow_init :: ema where
+  \<open>ema_slow_init \<equiv> ema_init 429450\<close>
+
+
+end
