Weidenbach_Book/IsaSAT/IsaSAT_Options.thy
@@ -1,0 +1,78 @@
+theory IsaSAT_Options
+imports IsaSAT_Literals
+begin
+
+section \<open>Options\<close>
+
+subsection \<open>Definition\<close>
+
+datatype opts =
+  IsaOptions (opts_restart: bool)
+  (opts_reduce: bool)
+  (opts_unbounded_mode: bool)
+  (opts_minimum_between_restart: \<open>64 word\<close>)
+  (opts_restart_coeff1: \<open>64 word\<close>)
+  (opts_restart_coeff2: nat)
+
+subsection \<open>Refinement\<close>
+
+type_synonym opts_ref =
+  \<open>bool \<times> bool \<times> bool \<times> 64 word \<times> 64 word \<times> nat\<close>
+
+definition opts_rel :: \<open>(opts_ref \<times> opts) set\<close> where
+  \<open>opts_rel = {(S, T). S = (opts_restart T, opts_reduce T, opts_unbounded_mode T,
+      opts_minimum_between_restart T, opts_restart_coeff1 T, opts_restart_coeff2 T)}\<close>
+
+fun opts_rel_restart :: \<open>opts_ref \<Rightarrow> bool\<close> where
+  \<open>opts_rel_restart (res, red, unbd, mini, res1, res2) = res\<close>
+
+lemma opts_rel_restart:
+  \<open>(opts_rel_restart, opts_restart) \<in> opts_rel \<rightarrow> bool_rel\<close>
+  by (auto simp: opts_rel_def intro!: frefI)
+
+
+fun opts_rel_reduce :: \<open>opts_ref \<Rightarrow> bool\<close> where
+  \<open>opts_rel_reduce (res, red, unbd, mini, res1, res2) = red\<close>
+
+lemma opts_rel_reduce:
+  \<open>(opts_rel_reduce, opts_reduce) \<in> opts_rel \<rightarrow> bool_rel\<close>
+  by (auto simp: opts_rel_def intro!: frefI)
+
+fun opts_rel_unbounded_mode :: \<open>opts_ref \<Rightarrow> bool\<close> where
+  \<open>opts_rel_unbounded_mode (res, red, unbd, mini, res1, res2) = unbd\<close>
+
+lemma opts_rel_unbounded_mode:
+  \<open>(opts_rel_unbounded_mode, opts_unbounded_mode) \<in> opts_rel \<rightarrow> bool_rel\<close>
+  by (auto simp: opts_rel_def intro!: frefI)
+
+fun opts_rel_miminum_between_restart :: \<open>opts_ref \<Rightarrow> 64 word\<close> where
+  \<open>opts_rel_miminum_between_restart (res, red, unbd, mini, res1, res2) = mini\<close>
+
+lemma opts_rel_miminum_between_restart:
+  \<open>(opts_rel_miminum_between_restart, opts_minimum_between_restart) \<in> opts_rel \<rightarrow> Id\<close>
+  by (auto simp: opts_rel_def intro!: frefI)
+
+fun opts_rel_restart_coeff1 :: \<open>opts_ref \<Rightarrow> 64 word\<close> where
+  \<open>opts_rel_restart_coeff1 (res, red, unbd, mini, res1, res2) = res1\<close>
+
+lemma opts_rel_restart_coeff1:
+  \<open>(opts_rel_restart_coeff1, opts_restart_coeff1) \<in> opts_rel \<rightarrow> Id\<close>
+  by (auto simp: opts_rel_def intro!: frefI)
+
+fun opts_rel_restart_coeff2 :: \<open>opts_ref \<Rightarrow> nat\<close> where
+  \<open>opts_rel_restart_coeff2 (res, red, unbd, mini, res1, res2) = res2\<close>
+
+lemma opts_rel_restart_coeff2:
+  \<open>(opts_rel_restart_coeff2, opts_restart_coeff2) \<in> opts_rel \<rightarrow> Id\<close>
+  by (auto simp: opts_rel_def intro!: frefI)
+
+lemma opts_rel_alt_defs:
+  \<open>RETURN o opts_rel_restart = (\<lambda>(res, red, unbd, mini, res1, res2). RETURN res)\<close>
+  \<open>RETURN o opts_rel_reduce = (\<lambda>(res, red, unbd, mini, res1, res2). RETURN red)\<close>
+  \<open>RETURN o opts_rel_unbounded_mode = (\<lambda>(res, red, unbd, mini, res1, res2). RETURN unbd)\<close>
+  \<open>RETURN o opts_rel_miminum_between_restart = (\<lambda>(res, red, unbd, mini, res1, res2). RETURN mini)\<close>
+  \<open>RETURN o opts_rel_restart_coeff1 = (\<lambda>(res, red, unbd, mini, res1, res2). RETURN res1)\<close>
+  \<open>RETURN o opts_rel_restart_coeff2 = (\<lambda>(res, red, unbd, mini, res1, res2). RETURN res2)\<close>
+  by (auto intro!: ext)
+
+end
