Weidenbach_Book/IsaSAT/IsaSAT_Options_LLVM.thy
@@ -1,0 +1,74 @@
+theory IsaSAT_Options_LLVM
+  imports IsaSAT_Options IsaSAT_Literals_LLVM
+begin
+
+type_synonym opts_assn = \<open>1 word \<times> 1 word \<times> 1 word \<times> 64 word \<times> 64 word \<times> 64 word\<close>
+
+definition opts_rel_assn :: \<open>opts_ref \<Rightarrow> _ \<Rightarrow> assn\<close> where
+  \<open>opts_rel_assn = bool1_assn \<times>\<^sub>a bool1_assn \<times>\<^sub>a bool1_assn \<times>\<^sub>a word_assn \<times>\<^sub>a word_assn \<times>\<^sub>a snat_assn' TYPE(64)\<close>
+
+sepref_def opts_rel_restart_code
+  is \<open>RETURN o opts_rel_restart\<close>
+  :: \<open>opts_rel_assn\<^sup>k \<rightarrow>\<^sub>a bool1_assn\<close>
+  unfolding opts_rel_alt_defs opts_rel_assn_def
+  by sepref
+
+
+sepref_def opts_rel_reduce_code
+  is \<open>RETURN o opts_rel_reduce\<close>
+  :: \<open>opts_rel_assn\<^sup>k \<rightarrow>\<^sub>a bool1_assn\<close>
+  unfolding opts_rel_alt_defs opts_rel_assn_def
+  by sepref
+
+sepref_def opts_rel_unbounded_mode_code
+  is \<open>RETURN o opts_rel_unbounded_mode\<close>
+  :: \<open>opts_rel_assn\<^sup>k \<rightarrow>\<^sub>a bool1_assn\<close>
+  unfolding opts_rel_alt_defs opts_rel_assn_def
+  by sepref
+
+sepref_def opts_rel_miminum_between_restart_code
+  is \<open>RETURN o opts_rel_miminum_between_restart\<close>
+  :: \<open>opts_rel_assn\<^sup>k \<rightarrow>\<^sub>a word_assn\<close>
+  unfolding opts_rel_alt_defs opts_rel_assn_def
+  by sepref
+
+sepref_def opts_rel_restart_coeff1_code
+  is \<open>RETURN o opts_rel_restart_coeff1\<close>
+  :: \<open>opts_rel_assn\<^sup>k \<rightarrow>\<^sub>a word_assn\<close>
+  unfolding opts_rel_alt_defs opts_rel_assn_def
+  by sepref
+
+sepref_def opts_rel_restart_coeff2_code
+  is \<open>RETURN o opts_rel_restart_coeff2\<close>
+  :: \<open>opts_rel_assn\<^sup>k \<rightarrow>\<^sub>a snat_assn' TYPE(64)\<close>
+  unfolding opts_rel_alt_defs opts_rel_assn_def
+  by sepref
+
+definition opts_assn :: \<open>opts \<Rightarrow> opts_assn \<Rightarrow> assn\<close> where
+  \<open>opts_assn = hr_comp opts_rel_assn opts_rel\<close>
+
+lemmas [sepref_fr_rules] =
+  opts_rel_restart_code.refine[FCOMP opts_rel_restart, unfolded opts_assn_def[symmetric]]
+  opts_rel_reduce_code.refine[FCOMP opts_rel_reduce, unfolded opts_assn_def[symmetric]]
+  opts_rel_unbounded_mode_code.refine[FCOMP opts_rel_unbounded_mode, unfolded opts_assn_def[symmetric]]
+  opts_rel_miminum_between_restart_code.refine[FCOMP opts_rel_miminum_between_restart, unfolded opts_assn_def[symmetric]]
+  opts_rel_restart_coeff1_code.refine[FCOMP opts_rel_restart_coeff1, unfolded opts_assn_def[symmetric]]
+  opts_rel_restart_coeff2_code.refine[FCOMP opts_rel_restart_coeff2, unfolded opts_assn_def[symmetric]]
+
+sepref_register opts_restart opts_reduce opts_minimum_between_restart opts_restart_coeff1
+  opts_restart_coeff2
+
+lemma opts_assn_assn_pure[safe_constraint_rules]: \<open>CONSTRAINT is_pure opts_assn\<close>
+  unfolding opts_assn_def opts_rel_assn_def
+  by solve_constraint
+
+lemmas [sepref_frame_free_rules] = mk_free_is_pure[OF opts_assn_assn_pure[unfolded CONSTRAINT_def]]
+
+experiment begin
+
+export_llvm
+  opts_rel_restart_code
+  opts_rel_reduce_code
+end
+
+end
