Weidenbach_Book/IsaSAT/IsaSAT_Rephase_State.thy
@@ -1,0 +1,72 @@
+theory IsaSAT_Rephase_State
+  imports IsaSAT_Rephase IsaSAT_Setup IsaSAT_Show
+begin
+
+definition rephase_heur :: \<open>64 word \<Rightarrow> restart_heuristics \<Rightarrow> restart_heuristics nres\<close> where
+  \<open>rephase_heur = (\<lambda>b (fast_ema, slow_ema, restart_info, wasted, \<phi>).
+    do {
+      \<phi> \<leftarrow> phase_rephase b \<phi>;
+      RETURN (fast_ema, slow_ema, restart_info, wasted, \<phi>)
+   })\<close>
+
+lemma rephase_heur_spec:
+  \<open>heuristic_rel \<A> heur \<Longrightarrow> rephase_heur b heur \<le>  \<Down>Id (SPEC(heuristic_rel \<A>))\<close>
+  unfolding rephase_heur_def
+  apply (refine_vcg phase_rephase_spec[THEN order_trans])
+  apply (auto simp: heuristic_rel_def)
+  done
+
+definition rephase_heur_st :: \<open>twl_st_wl_heur \<Rightarrow> twl_st_wl_heur nres\<close> where
+  \<open>rephase_heur_st = (\<lambda>(M', arena, D', j, W', vm, clvls, cach, lbd, outl, stats, heur,
+       vdom, avdom, lcount, opts, old_arena). do {
+      let b = current_restart_phase heur;
+      heur \<leftarrow> rephase_heur b heur;
+      let _ = isasat_print_progress (current_rephasing_phase heur) b stats lcount;
+      RETURN (M', arena, D', j, W', vm, clvls, cach, lbd, outl, stats, heur,
+       vdom, avdom, lcount, opts, old_arena)
+   })\<close>
+
+lemma rephase_heur_st_spec:
+  \<open>(S, S') \<in> twl_st_heur \<Longrightarrow> rephase_heur_st S \<le> SPEC(\<lambda>S. (S, S') \<in> twl_st_heur)\<close>
+  unfolding rephase_heur_st_def
+  apply (cases S')
+  apply (refine_vcg rephase_heur_spec[THEN order_trans, of \<open>all_atms_st S'\<close>])
+  apply (simp_all add:  twl_st_heur_def)
+  done
+
+definition save_rephase_heur :: \<open>nat \<Rightarrow> restart_heuristics \<Rightarrow> restart_heuristics nres\<close> where
+  \<open>save_rephase_heur = (\<lambda>n (fast_ema, slow_ema, restart_info, wasted, \<phi>).
+    do {
+      \<phi> \<leftarrow> phase_save_phase n \<phi>;
+      RETURN (fast_ema, slow_ema, restart_info, wasted, \<phi>)
+   })\<close>
+
+lemma save_phase_heur_spec:
+  \<open>heuristic_rel \<A> heur \<Longrightarrow> save_rephase_heur n heur \<le>  \<Down>Id (SPEC(heuristic_rel \<A>))\<close>
+  unfolding save_rephase_heur_def
+  apply (refine_vcg phase_save_phase_spec[THEN order_trans])
+  apply (auto simp: heuristic_rel_def)
+  done
+
+
+definition save_phase_st :: \<open>twl_st_wl_heur \<Rightarrow> twl_st_wl_heur nres\<close> where
+  \<open>save_phase_st = (\<lambda>(M', arena, D', j, W', vm, clvls, cach, lbd, outl, stats, heur,
+       vdom, avdom, lcount, opts, old_arena). do {
+      ASSERT(isa_length_trail_pre M');
+      let n = isa_length_trail M';
+      heur \<leftarrow> save_rephase_heur n heur;
+      RETURN (M', arena, D', j, W', vm, clvls, cach, lbd, outl, stats, heur,
+       vdom, avdom, lcount, opts, old_arena)
+   })\<close>
+
+lemma save_phase_st_spec:
+  \<open>(S, S') \<in> twl_st_heur \<Longrightarrow> save_phase_st S \<le> SPEC(\<lambda>S. (S, S') \<in> twl_st_heur)\<close>
+  unfolding save_phase_st_def
+  apply (cases S')
+  apply (refine_vcg save_phase_heur_spec[THEN order_trans, of \<open>all_atms_st S'\<close>])
+  apply (simp_all add:  twl_st_heur_def isa_length_trail_pre)
+  apply (rule isa_length_trail_pre)
+  apply blast
+  done
+
+end
