Weidenbach_Book/IsaSAT/IsaSAT_Rephase_State_LLVM.thy
@@ -1,0 +1,63 @@
+theory IsaSAT_Rephase_State_LLVM
+imports
+  IsaSAT_Rephase_State IsaSAT_Rephase_LLVM IsaSAT_Show_LLVM
+begin
+
+sepref_def save_phase_heur_impl
+  is \<open>uncurry save_rephase_heur\<close>
+  ::  \<open>sint64_nat_assn\<^sup>k *\<^sub>a heuristic_assn\<^sup>d \<rightarrow>\<^sub>a heuristic_assn\<close>
+  supply [[goals_limit=1]]
+  unfolding save_rephase_heur_def heuristic_assn_def
+  by sepref
+
+
+sepref_def save_phase_heur_st
+  is save_phase_st
+  ::  \<open>isasat_bounded_assn\<^sup>d \<rightarrow>\<^sub>a isasat_bounded_assn\<close>
+  supply [[goals_limit=1]]
+  unfolding save_phase_st_def isasat_bounded_assn_def
+  by sepref
+
+sepref_def phase_save_rephase_impl
+  is \<open>uncurry phase_rephase\<close>
+  :: \<open>word_assn\<^sup>k *\<^sub>a phase_heur_assn\<^sup>d \<rightarrow>\<^sub>a phase_heur_assn\<close>
+  unfolding phase_rephase_def copy_phase2_def[symmetric]
+  by sepref
+
+
+sepref_def rephase_heur_impl
+  is \<open>uncurry rephase_heur\<close>
+  :: \<open>word_assn\<^sup>k *\<^sub>a heuristic_assn\<^sup>d \<rightarrow>\<^sub>a heuristic_assn\<close>
+  unfolding rephase_heur_def heuristic_assn_def
+  by sepref
+
+lemma current_rephasing_phase_alt_def:
+  \<open>RETURN o current_rephasing_phase =
+    (\<lambda>(fast_ema, slow_ema, res_info, wasted,
+      (\<phi>, target_assigned, target, best_assigned, best, end_of_phase, curr_phase, length_phase)).
+      RETURN curr_phase)\<close>
+  unfolding current_rephasing_phase_def
+    phase_current_rephasing_phase_def
+  by (auto intro!: ext)
+
+sepref_def current_rephasing_phase
+  is \<open>RETURN o current_rephasing_phase\<close>
+  :: \<open>heuristic_assn\<^sup>k \<rightarrow>\<^sub>a word64_assn\<close>
+  unfolding current_rephasing_phase_alt_def heuristic_assn_def
+  by sepref
+
+sepref_register rephase_heur
+sepref_def rephase_heur_st_impl
+  is rephase_heur_st
+  ::  \<open>isasat_bounded_assn\<^sup>d \<rightarrow>\<^sub>a isasat_bounded_assn\<close>
+  unfolding rephase_heur_st_def isasat_bounded_assn_def
+  by sepref
+
+
+experiment
+begin
+export_llvm rephase_heur_st_impl
+  save_phase_heur_st
+end
+
+end
