Weidenbach_Book/IsaSAT/IsaSAT_Restart_Heuristics_LLVM.thy
@@ -1,6 +1,6 @@
 theory IsaSAT_Restart_Heuristics_LLVM
   imports IsaSAT_Restart_Heuristics IsaSAT_Setup_LLVM
-     IsaSAT_VMTF_State_LLVM IsaSAT_Rephase_LLVM
+     IsaSAT_VMTF_State_LLVM IsaSAT_Rephase_State_LLVM
      IsaSAT_Arena_Sorting_LLVM
 begin
 
@@ -294,26 +294,6 @@ sepref_def restart_required_heur_fast_code
   apply (annot_snat_const \<open>TYPE(64)\<close>)
   by sepref
 
-sepref_register isa_trail_nth isasat_trail_nth_st
-
-sepref_def isasat_trail_nth_st_code
-  is \<open>uncurry isasat_trail_nth_st\<close>
-  :: \<open>isasat_bounded_assn\<^sup>k *\<^sub>a sint64_nat_assn\<^sup>k \<rightarrow>\<^sub>a unat_lit_assn\<close>
-  supply [[goals_limit=1]]
-  unfolding isasat_trail_nth_st_alt_def isasat_bounded_assn_def
-  by sepref
-
-
-
-sepref_register get_the_propagation_reason_pol_st
-
-sepref_def get_the_propagation_reason_pol_st_code
-  is \<open>uncurry get_the_propagation_reason_pol_st\<close>
-  :: \<open>isasat_bounded_assn\<^sup>k *\<^sub>a unat_lit_assn\<^sup>k \<rightarrow>\<^sub>a snat_option_assn' TYPE(64)\<close>
-  supply [[goals_limit=1]]
-  unfolding get_the_propagation_reason_pol_st_alt_def isasat_bounded_assn_def
-  by sepref
-
 sepref_register isasat_replace_annot_in_trail
 sepref_def isasat_replace_annot_in_trail_code
   is \<open>uncurry2 isasat_replace_annot_in_trail\<close>
@@ -383,12 +363,6 @@ lemma remove_one_annot_true_clause_imp_wl_D_heurI:
        learned_clss_count a2' \<le> uint64_max\<close>
   by (auto simp: isasat_fast_def remove_one_annot_true_clause_imp_wl_D_heur_inv_def)
 
-sepref_def empty_US_heur_code
-  is \<open>RETURN o empty_US_heur\<close>
-  :: \<open>isasat_bounded_assn\<^sup>d \<rightarrow>\<^sub>a isasat_bounded_assn\<close>
-  unfolding empty_US_heur_def isasat_bounded_assn_def
-  by sepref
-
 sepref_def remove_one_annot_true_clause_imp_wl_D_heur_code
   is \<open>remove_one_annot_true_clause_imp_wl_D_heur\<close>
   :: \<open>[\<lambda>S. length (get_clauses_wl_heur S) \<le> sint64_max \<and> 
@@ -400,180 +374,8 @@ sepref_def remove_one_annot_true_clause_imp_wl_D_heur_code
   apply (annot_unat_const \<open>TYPE(32)\<close>)
   by sepref
 
-
-lemma length_ll[def_pat_rules]: \<open>length_ll$xs$i \<equiv> op_list_list_llen$xs$i\<close>
-  by (auto simp: length_ll_def)
-
-lemma [def_pat_rules]: \<open>nth_rll \<equiv> op_list_list_idx\<close>
-  by (auto simp: nth_rll_def[abs_def] op_list_list_idx_def intro!: ext)
-
-sepref_register length_ll extra_information_mark_to_delete nth_rll
-  LEARNED
-
-lemma isasat_GC_clauses_prog_copy_wl_entry_alt_def:
-\<open>isasat_GC_clauses_prog_copy_wl_entry = (\<lambda>N0 W A (N', vdm, avdm). do {
-    ASSERT(nat_of_lit A < length W);
-    ASSERT(length (W ! nat_of_lit A) \<le> length N0);
-    let le = length (W ! nat_of_lit A);
-    (i, N, N', vdm, avdm) \<leftarrow> WHILE\<^sub>T
-      (\<lambda>(i, N, N', vdm, avdm). i < le)
-      (\<lambda>(i, N, (N', vdm, avdm)). do {
-        ASSERT(i < length (W ! nat_of_lit A));
-        let (C, _, _) = (W ! nat_of_lit A ! i);
-        ASSERT(arena_is_valid_clause_vdom N C);
-        let st = arena_status N C;
-        if st \<noteq> DELETED then do {
-          ASSERT(arena_is_valid_clause_idx N C);
-          ASSERT(length N' + (if arena_length N C > 4 then MAX_HEADER_SIZE else MIN_HEADER_SIZE) + arena_length N C \<le> length N0);
-          ASSERT(length N = length N0);
-          ASSERT(length vdm < length N0);
-          ASSERT(length avdm < length N0);
-          let D = length N' + (if arena_length N C > 4 then MAX_HEADER_SIZE else MIN_HEADER_SIZE);
-          N' \<leftarrow> fm_mv_clause_to_new_arena C N N';
-          ASSERT(mark_garbage_pre (N, C));
-	  RETURN (i+1, extra_information_mark_to_delete N C, N', vdm @ [D],
-             (if st = LEARNED then avdm @ [D] else avdm))
-        } else RETURN (i+1, N, (N', vdm, avdm))
-      }) (0, N0, (N', vdm, avdm));
-    RETURN (N, (N', vdm, avdm))
-  })\<close>
-proof -
-  have H: \<open>(let (a, _, _) = c in f a) = (let a = fst c in f a)\<close> for a c f
-    by (cases c) (auto simp: Let_def)
-  show ?thesis
-    unfolding isasat_GC_clauses_prog_copy_wl_entry_def H
-    ..
-qed
-
-sepref_def isasat_GC_clauses_prog_copy_wl_entry_code
-  is \<open>uncurry3 isasat_GC_clauses_prog_copy_wl_entry\<close>
-  :: \<open>[\<lambda>(((N, _), _), _). length N \<le> sint64_max]\<^sub>a
-     arena_fast_assn\<^sup>d *\<^sub>a watchlist_fast_assn\<^sup>k *\<^sub>a unat_lit_assn\<^sup>k *\<^sub>a
-         (arena_fast_assn \<times>\<^sub>a vdom_fast_assn \<times>\<^sub>a vdom_fast_assn)\<^sup>d \<rightarrow>
-     (arena_fast_assn \<times>\<^sub>a (arena_fast_assn \<times>\<^sub>a vdom_fast_assn \<times>\<^sub>a vdom_fast_assn))\<close>
-  supply [[goals_limit=1]] if_splits[split] length_ll_def[simp]
-  unfolding isasat_GC_clauses_prog_copy_wl_entry_alt_def nth_rll_def[symmetric]
-    length_ll_def[symmetric] if_conn(4)
-  apply (annot_snat_const \<open>TYPE(64)\<close>)
-  by sepref
-
-sepref_register isasat_GC_clauses_prog_copy_wl_entry
-
-lemma shorten_taken_op_list_list_take:
-  \<open>W[L := []] = op_list_list_take W L 0\<close>
-  by (auto simp:)
-
-sepref_def isasat_GC_clauses_prog_single_wl_code
-  is \<open>uncurry3 isasat_GC_clauses_prog_single_wl\<close>
-  :: \<open>[\<lambda>(((N, _), _), A). A \<le> uint32_max div 2 \<and> length N \<le> sint64_max]\<^sub>a
-     arena_fast_assn\<^sup>d *\<^sub>a (arena_fast_assn \<times>\<^sub>a vdom_fast_assn \<times>\<^sub>a vdom_fast_assn)\<^sup>d *\<^sub>a watchlist_fast_assn\<^sup>d *\<^sub>a atom_assn\<^sup>k \<rightarrow>
-     (arena_fast_assn \<times>\<^sub>a (arena_fast_assn \<times>\<^sub>a vdom_fast_assn \<times>\<^sub>a vdom_fast_assn) \<times>\<^sub>a watchlist_fast_assn)\<close>
-  supply [[goals_limit=1]]
-  unfolding isasat_GC_clauses_prog_single_wl_def
-    shorten_taken_op_list_list_take
-  apply (annot_snat_const \<open>TYPE(64)\<close>)
-  by sepref
-
-
-definition isasat_GC_clauses_prog_wl2' where
-  \<open>isasat_GC_clauses_prog_wl2' ns fst' = (isasat_GC_clauses_prog_wl2 (ns, fst'))\<close>
-
-sepref_register isasat_GC_clauses_prog_wl2 isasat_GC_clauses_prog_single_wl
-sepref_def isasat_GC_clauses_prog_wl2_code
-  is \<open>uncurry2 isasat_GC_clauses_prog_wl2'\<close>
-  :: \<open>[\<lambda>((_, _), (N, _)). length N \<le> sint64_max]\<^sub>a
-     (array_assn vmtf_node_assn)\<^sup>k *\<^sub>a (atom.option_assn)\<^sup>k *\<^sub>a
-     (arena_fast_assn \<times>\<^sub>a (arena_fast_assn \<times>\<^sub>a vdom_fast_assn \<times>\<^sub>a vdom_fast_assn) \<times>\<^sub>a watchlist_fast_assn)\<^sup>d \<rightarrow>
-     (arena_fast_assn \<times>\<^sub>a (arena_fast_assn \<times>\<^sub>a vdom_fast_assn \<times>\<^sub>a vdom_fast_assn) \<times>\<^sub>a watchlist_fast_assn)\<close>
-  supply [[goals_limit=1]]
-  unfolding isasat_GC_clauses_prog_wl2_def isasat_GC_clauses_prog_wl2'_def prod.case
-    atom.fold_option
-  apply (rewrite at \<open> _ ! _\<close> annot_index_of_atm)
-  by sepref
-
 (*TODO Move*)
-sepref_def set_zero_wasted_impl
-  is \<open>RETURN o set_zero_wasted\<close>
-  :: \<open>heuristic_assn\<^sup>d \<rightarrow>\<^sub>a heuristic_assn\<close>
-  unfolding heuristic_assn_def set_zero_wasted_def
-  by sepref
 
-sepref_register isasat_GC_clauses_prog_wl isasat_GC_clauses_prog_wl2' rewatch_heur_st
-sepref_def isasat_GC_clauses_prog_wl_code
-  is \<open>isasat_GC_clauses_prog_wl\<close>
-  :: \<open>[\<lambda>S. length (get_clauses_wl_heur S) \<le> sint64_max]\<^sub>a isasat_bounded_assn\<^sup>d \<rightarrow> isasat_bounded_assn\<close>
-  supply [[goals_limit=1]]
-  unfolding isasat_GC_clauses_prog_wl_def isasat_bounded_assn_def
-     isasat_GC_clauses_prog_wl2'_def[symmetric] vmtf_remove_assn_def
-    atom.fold_option fold_tuple_optimizations
-  apply (annot_snat_const \<open>TYPE(64)\<close>)
-  by sepref
-
-lemma rewatch_heur_st_pre_alt_def:
-  \<open>rewatch_heur_st_pre S \<longleftrightarrow> (\<forall>i \<in> set (get_vdom S). i \<le> sint64_max)\<close>
-  by (auto simp: rewatch_heur_st_pre_def all_set_conv_nth)
-
-sepref_def rewatch_heur_st_code
-  is \<open>rewatch_heur_st\<close>
-  :: \<open>[\<lambda>S. rewatch_heur_st_pre S \<and> length (get_clauses_wl_heur S) \<le> sint64_max]\<^sub>a isasat_bounded_assn\<^sup>d \<rightarrow> isasat_bounded_assn\<close>
-  supply [[goals_limit=1]]  append_ll_def[simp]
-  unfolding isasat_GC_clauses_prog_wl_def isasat_bounded_assn_def
-    rewatch_heur_st_def Let_def rewatch_heur_st_pre_alt_def
-  by sepref
-
-sepref_register isasat_GC_clauses_wl_D
-
-lemma get_clauses_wl_heur_empty_US[simp]:
-    \<open>get_clauses_wl_heur (empty_US_heur xc) = get_clauses_wl_heur xc\<close> and
-  get_vdom_empty_US[simp]:
-    \<open>get_vdom (empty_US_heur xc) = get_vdom xc\<close>
-  by (cases xc; auto simp: empty_US_heur_def; fail)+
-
-sepref_def isasat_GC_clauses_wl_D_code
-  is \<open>isasat_GC_clauses_wl_D\<close>
-  :: \<open>[\<lambda>S. length (get_clauses_wl_heur S) \<le> sint64_max]\<^sub>a
-      isasat_bounded_assn\<^sup>d \<rightarrow> isasat_bounded_assn\<close>
-  supply [[goals_limit=1]] isasat_GC_clauses_wl_D_rewatch_pre[intro!]
-  unfolding isasat_GC_clauses_wl_D_def
-  by sepref
-
-sepref_register number_clss_to_keep
-
-sepref_register access_vdom_at
-
-lemma [sepref_fr_rules]:
-  \<open>(return o id, RETURN o unat) \<in> word64_assn\<^sup>k \<rightarrow>\<^sub>a uint64_nat_assn\<close>
-proof -
-  have [simp]: \<open>(\<lambda>s. \<exists>xa. (\<up>(xa = unat x) \<and>* \<up>(xa = unat x)) s) = \<up>True\<close>
-    by (intro ext)
-     (auto intro!: exI[of _ \<open>unat x\<close>] simp: pure_true_conv pure_part_pure_eq pred_lift_def
-      simp flip: import_param_3)
-  show ?thesis
-    apply sepref_to_hoare
-    apply (vcg)
-    apply (auto simp: unat_rel_def unat.rel_def br_def pred_lift_def ENTAILS_def pure_true_conv simp flip: import_param_3 pure_part_def)
-    done
-qed
-
-sepref_def number_clss_to_keep_fast_code
-  is \<open>number_clss_to_keep_impl\<close>
-  :: \<open>isasat_bounded_assn\<^sup>k \<rightarrow>\<^sub>a sint64_nat_assn\<close>
-  supply [[goals_limit = 1]]
-  unfolding number_clss_to_keep_impl_def isasat_bounded_assn_def
-    fold_tuple_optimizations
-  apply (rewrite at \<open>If _ _ \<hole>\<close> annot_unat_snat_conv)
-  apply (rewrite at \<open>If (\<hole> \<le>_)\<close> annot_snat_unat_conv)
-  by sepref
-
-lemma number_clss_to_keep_impl_number_clss_to_keep:
-  \<open>(number_clss_to_keep_impl, number_clss_to_keep) \<in> Sepref_Rules.freft Id (\<lambda>_. \<langle>nat_rel\<rangle>nres_rel)\<close>
-  by (auto simp: number_clss_to_keep_impl_def number_clss_to_keep_def Let_def intro!: Sepref_Rules.frefI nres_relI)
-
-lemma number_clss_to_keep_fast_code_refine[sepref_fr_rules]:
-  \<open>(number_clss_to_keep_fast_code, number_clss_to_keep) \<in> (isasat_bounded_assn)\<^sup>k \<rightarrow>\<^sub>a snat_assn\<close>
-  using hfcomp[OF number_clss_to_keep_fast_code.refine
-    number_clss_to_keep_impl_number_clss_to_keep, simplified]
-  by auto
 
 
 sepref_def mark_clauses_as_unused_wl_D_heur_fast_code
@@ -591,7 +393,6 @@ experiment
 begin
   export_llvm restart_required_heur_fast_code
     access_vdom_at_fast_code
-    isasat_GC_clauses_wl_D_code
 end
 
 end
