Weidenbach_Book/IsaSAT/IsaSAT_Stats.thy
@@ -1,0 +1,259 @@
+theory IsaSAT_Stats
+  imports IsaSAT_Literals IsaSAT_EMA IsaSAT_Rephase
+begin
+
+section \<open>Statistics\<close>
+
+text \<open>
+We do some statistics on the run.
+
+NB: the statistics are not proven correct (especially they might
+overflow), there are just there to look for regressions, do some comparisons (e.g., to conclude that
+we are propagating slower than the other solvers), or to test different option combination.
+\<close>
+type_synonym stats = \<open>64 word \<times> 64 word \<times> 64 word \<times> 64 word \<times> 64 word \<times> 64 word \<times> 64 word \<times> ema\<close>
+
+
+definition incr_propagation :: \<open>stats \<Rightarrow> stats\<close> where
+  \<open>incr_propagation = (\<lambda>(propa, confl, dec). (propa + 1, confl, dec))\<close>
+
+definition incr_conflict :: \<open>stats \<Rightarrow> stats\<close> where
+  \<open>incr_conflict = (\<lambda>(propa, confl, dec). (propa, confl + 1, dec))\<close>
+
+definition incr_decision :: \<open>stats \<Rightarrow> stats\<close> where
+  \<open>incr_decision = (\<lambda>(propa, confl, dec, res). (propa, confl, dec + 1, res))\<close>
+
+definition incr_restart :: \<open>stats \<Rightarrow> stats\<close> where
+  \<open>incr_restart = (\<lambda>(propa, confl, dec, res, lres). (propa, confl, dec, res + 1, lres))\<close>
+
+definition incr_lrestart :: \<open>stats \<Rightarrow> stats\<close> where
+  \<open>incr_lrestart = (\<lambda>(propa, confl, dec, res, lres, uset). (propa, confl, dec, res, lres + 1, uset))\<close>
+
+definition incr_uset :: \<open>stats \<Rightarrow> stats\<close> where
+  \<open>incr_uset = (\<lambda>(propa, confl, dec, res, lres, (uset, gcs)). (propa, confl, dec, res, lres, uset + 1, gcs))\<close>
+
+definition incr_GC :: \<open>stats \<Rightarrow> stats\<close> where
+  \<open>incr_GC = (\<lambda>(propa, confl, dec, res, lres, uset, gcs, lbds). (propa, confl, dec, res, lres, uset, gcs + 1, lbds))\<close>
+
+definition add_lbd :: \<open>32 word \<Rightarrow> stats \<Rightarrow> stats\<close> where
+  \<open>add_lbd lbd = (\<lambda>(propa, confl, dec, res, lres, uset, gcs, lbds). (propa, confl, dec, res, lres, uset, gcs, ema_update (unat lbd) lbds))\<close>
+
+
+section \<open>Information related to restarts\<close>
+
+definition NORMAL_PHASE :: \<open>64 word\<close> where
+  \<open>NORMAL_PHASE = 0\<close>
+
+definition QUIET_PHASE :: \<open>64 word\<close> where
+  \<open>QUIET_PHASE = 1\<close>
+
+definition DEFAULT_INIT_PHASE :: \<open>64 word\<close> where
+  \<open>DEFAULT_INIT_PHASE = 10000\<close>
+
+
+type_synonym restart_info = \<open>64 word \<times> 64 word \<times> 64 word \<times> 64 word \<times> 64 word\<close>
+
+definition incr_conflict_count_since_last_restart :: \<open>restart_info \<Rightarrow> restart_info\<close> where
+  \<open>incr_conflict_count_since_last_restart = (\<lambda>(ccount, ema_lvl, restart_phase, end_of_phase, length_phase).
+    (ccount + 1, ema_lvl, restart_phase, end_of_phase, length_phase))\<close>
+
+definition restart_info_update_lvl_avg :: \<open>32 word \<Rightarrow> restart_info \<Rightarrow> restart_info\<close> where
+  \<open>restart_info_update_lvl_avg = (\<lambda>lvl (ccount, ema_lvl). (ccount, ema_lvl))\<close>
+
+definition restart_info_init :: \<open>restart_info\<close> where
+  \<open>restart_info_init = (0, 0, NORMAL_PHASE, DEFAULT_INIT_PHASE, 1000)\<close>
+
+definition restart_info_restart_done :: \<open>restart_info \<Rightarrow> restart_info\<close> where
+  \<open>restart_info_restart_done = (\<lambda>(ccount, lvl_avg). (0, lvl_avg))\<close>
+
+
+
+section \<open>Heuristics\<close>
+
+type_synonym restart_heuristics = \<open>ema \<times> ema \<times> restart_info \<times> 64 word \<times> phase_save_heur\<close>
+
+fun fast_ema_of :: \<open>restart_heuristics \<Rightarrow> ema\<close> where
+  \<open>fast_ema_of (fast_ema, slow_ema, restart_info, wasted, \<phi>) = fast_ema\<close>
+
+fun slow_ema_of :: \<open>restart_heuristics \<Rightarrow> ema\<close> where
+  \<open>slow_ema_of (fast_ema, slow_ema, restart_info, wasted, \<phi>) = slow_ema\<close>
+
+fun restart_info_of :: \<open>restart_heuristics \<Rightarrow> restart_info\<close> where
+  \<open>restart_info_of (fast_ema, slow_ema, restart_info, wasted, \<phi>) = restart_info\<close>
+
+fun current_restart_phase :: \<open>restart_heuristics \<Rightarrow> 64 word\<close> where
+  \<open>current_restart_phase (fast_ema, slow_ema, (ccount, ema_lvl, restart_phase, end_of_phase), wasted, \<phi>) =
+    restart_phase\<close>
+
+fun incr_restart_phase :: \<open>restart_heuristics \<Rightarrow> restart_heuristics\<close> where
+  \<open>incr_restart_phase (fast_ema, slow_ema, (ccount, ema_lvl, restart_phase, end_of_phase), wasted, \<phi>) =
+    (fast_ema, slow_ema, (ccount, ema_lvl, restart_phase XOR 1, end_of_phase), wasted, \<phi>)\<close>
+
+fun incr_wasted :: \<open>64 word \<Rightarrow> restart_heuristics \<Rightarrow> restart_heuristics\<close> where
+  \<open>incr_wasted waste (fast_ema, slow_ema, res_info, wasted, \<phi>) =
+    (fast_ema, slow_ema, res_info, wasted + waste, \<phi>)\<close>
+
+fun set_zero_wasted :: \<open>restart_heuristics \<Rightarrow> restart_heuristics\<close> where
+  \<open>set_zero_wasted (fast_ema, slow_ema, res_info, wasted, \<phi>) =
+    (fast_ema, slow_ema, res_info, 0, \<phi>)\<close>
+
+fun wasted_of :: \<open>restart_heuristics \<Rightarrow> 64 word\<close> where
+  \<open>wasted_of (fast_ema, slow_ema, res_info, wasted, \<phi>) = wasted\<close>
+
+definition heuristic_rel :: \<open>nat multiset \<Rightarrow> restart_heuristics \<Rightarrow> bool\<close> where
+  \<open>heuristic_rel \<A> = (\<lambda>(fast_ema, slow_ema, res_info, wasted, \<phi>). phase_save_heur_rel \<A> \<phi>)\<close>
+
+definition save_phase_heur :: \<open>nat \<Rightarrow> bool \<Rightarrow> restart_heuristics \<Rightarrow> restart_heuristics\<close> where
+\<open>save_phase_heur L b = (\<lambda>(fast_ema, slow_ema, res_info, wasted, (\<phi>, target, best)).
+    (fast_ema, slow_ema, res_info, wasted, (\<phi>[L := b], target, best)))\<close>
+
+definition save_phase_heur_pre :: \<open>nat \<Rightarrow> bool \<Rightarrow> restart_heuristics \<Rightarrow> bool\<close> where
+\<open>save_phase_heur_pre L b = (\<lambda>(fast_ema, slow_ema, res_info, wasted, (\<phi>, _)). L < length \<phi>)\<close>
+
+definition mop_save_phase_heur :: \<open>nat \<Rightarrow> bool \<Rightarrow> restart_heuristics \<Rightarrow> restart_heuristics nres\<close> where
+\<open>mop_save_phase_heur L b heur = do {
+   ASSERT(save_phase_heur_pre L b heur);
+   RETURN (save_phase_heur L b heur)
+}\<close>
+
+definition get_saved_phase_heur_pre :: \<open>nat \<Rightarrow> restart_heuristics \<Rightarrow> bool\<close> where
+\<open>get_saved_phase_heur_pre L = (\<lambda>(fast_ema, slow_ema, res_info, wasted, (\<phi>, _)). L < length \<phi>)\<close>
+
+definition get_saved_phase_heur :: \<open>nat \<Rightarrow> restart_heuristics \<Rightarrow> bool\<close> where
+\<open>get_saved_phase_heur L = (\<lambda>(fast_ema, slow_ema, res_info, wasted, (\<phi>, _)). \<phi>!L)\<close>
+
+definition current_rephasing_phase :: \<open>restart_heuristics \<Rightarrow> 64 word\<close> where
+\<open>current_rephasing_phase = (\<lambda>(fast_ema, slow_ema, res_info, wasted, \<phi>). phase_current_rephasing_phase \<phi>)\<close>
+
+definition mop_get_saved_phase_heur :: \<open>nat \<Rightarrow> restart_heuristics \<Rightarrow> bool nres\<close> where
+\<open>mop_get_saved_phase_heur L heur = do {
+   ASSERT(get_saved_phase_heur_pre L heur);
+   RETURN (get_saved_phase_heur L heur)
+}\<close>
+
+
+definition end_of_rephasing_phase_heur :: \<open>restart_heuristics \<Rightarrow> 64 word\<close> where
+  \<open>end_of_rephasing_phase_heur =
+    (\<lambda>(fast_ema, slow_ema, res_info, wasted, phasing). end_of_rephasing_phase phasing)\<close>
+
+
+lemma heuristic_relI[intro!]:
+  \<open>heuristic_rel \<A> heur \<Longrightarrow> heuristic_rel \<A> (incr_wasted wast heur)\<close>
+  \<open>heuristic_rel \<A> heur \<Longrightarrow> heuristic_rel \<A> (set_zero_wasted heur)\<close>
+  \<open>heuristic_rel \<A> heur \<Longrightarrow> heuristic_rel \<A> (incr_restart_phase heur)\<close>
+  \<open>heuristic_rel \<A> heur \<Longrightarrow> heuristic_rel \<A> (save_phase_heur L b heur)\<close>
+  by (clarsimp_all simp: heuristic_rel_def save_phase_heur_def phase_save_heur_rel_def phase_saving_def)
+
+lemma save_phase_heur_preI:
+  \<open>heuristic_rel \<A> heur \<Longrightarrow> a \<in># \<A> \<Longrightarrow> save_phase_heur_pre a b heur\<close>
+  by (auto simp: heuristic_rel_def phase_saving_def save_phase_heur_pre_def
+     phase_save_heur_rel_def atms_of_\<L>\<^sub>a\<^sub>l\<^sub>l_\<A>\<^sub>i\<^sub>n)
+
+subsection \<open>Number of clauses\<close>
+
+type_synonym clss_size = \<open>nat \<times> nat \<times> nat\<close>
+
+definition clss_size
+  :: \<open>'v clauses_l \<Rightarrow> 'v clauses \<Rightarrow> 'v clauses \<Rightarrow> 'v clauses \<Rightarrow> 'v clauses \<Rightarrow> clss_size\<close>
+where
+  \<open>clss_size N NE UE NS US =
+     (size (learned_clss_lf N), size UE, size US)\<close>
+
+definition clss_size_lcount :: \<open>clss_size \<Rightarrow> nat\<close> where
+  \<open>clss_size_lcount = (\<lambda>(lcount, lcountUE, lcountUS). lcount)\<close>
+
+definition clss_size_lcountUE :: \<open>clss_size \<Rightarrow> nat\<close> where
+  \<open>clss_size_lcountUE = (\<lambda>(lcount, lcountUE, lcountUS). lcountUE)\<close>
+
+definition clss_size_lcountUS :: \<open>clss_size \<Rightarrow> nat\<close> where
+  \<open>clss_size_lcountUS = (\<lambda>(lcount, lcountUE, lcountUS). lcountUS)\<close>
+
+definition clss_size_incr_lcount :: \<open>clss_size \<Rightarrow> clss_size\<close> where
+  \<open>clss_size_incr_lcount =
+     (\<lambda>(lcount, lcountUE, lcountUS). (lcount + 1, lcountUE, lcountUS))\<close>
+
+definition clss_size_decr_lcount :: \<open>clss_size \<Rightarrow> clss_size\<close> where
+  \<open>clss_size_decr_lcount =
+     (\<lambda>(lcount, lcountUE, lcountUS). (lcount - 1, lcountUE, lcountUS))\<close>
+
+definition clss_size_incr_lcountUE :: \<open>clss_size \<Rightarrow> clss_size\<close> where
+  \<open>clss_size_incr_lcountUE =
+     (\<lambda>(lcount, lcountUE, lcountUS). (lcount, lcountUE + 1, lcountUS))\<close>
+
+definition clss_size_incr_lcountUS :: \<open>clss_size \<Rightarrow> clss_size\<close> where
+  \<open>clss_size_incr_lcountUS =
+     (\<lambda>(lcount, lcountUE, lcountUS). (lcount, lcountUE, lcountUS + 1))\<close>
+
+definition clss_size_resetUS :: \<open>clss_size \<Rightarrow> clss_size\<close> where
+  \<open>clss_size_resetUS =
+     (\<lambda>(lcount, lcountUE, lcountUS). (lcount, lcountUE, 0))\<close>
+
+definition clss_size_allcount :: \<open>clss_size \<Rightarrow> nat\<close> where
+  \<open>clss_size_allcount =
+    (\<lambda>(lcount, lcountUE, lcountUS). lcount + lcountUE + lcountUS)\<close>
+
+lemma clss_size_add_simp[simp]:
+  \<open>clss_size N NE (add_mset D UE) NS US = clss_size_incr_lcountUE (clss_size N NE UE NS US)\<close>
+  \<open>clss_size N (add_mset C NE) UE NS US = clss_size N NE UE NS US\<close>
+  \<open>clss_size N NE UE (add_mset C NS) US = clss_size N NE UE NS US\<close>
+  by (auto simp: clss_size_def ran_m_fmdrop_If clss_size_decr_lcount_def
+    clss_size_incr_lcountUE_def size_remove1_mset_If clss_size_resetUS_def)
+
+lemma clss_size_upd_simp[simp]:
+  \<open>C \<in># dom_m N \<Longrightarrow>  clss_size (N(C \<hookrightarrow> C')) NE UE NS US = clss_size N NE UE NS US\<close>
+  \<open>C \<notin># dom_m N \<Longrightarrow> \<not>snd D \<Longrightarrow> clss_size (fmupd C D N) NE UE NS US = clss_size_incr_lcount (clss_size N NE UE NS US)\<close>
+  \<open>C \<notin># dom_m N \<Longrightarrow> snd D \<Longrightarrow> clss_size (fmupd C D N) NE UE NS US = (clss_size N NE UE NS US)\<close>
+  by (auto simp: clss_size_def learned_clss_l_fmupd_if clss_size_incr_lcount_def)
+
+lemma clss_size_del_simp[simp]:
+  \<open>C \<in># dom_m N \<Longrightarrow> \<not>irred N C \<Longrightarrow> clss_size (fmdrop C N) NE UE NS US = clss_size_decr_lcount (clss_size N NE UE NS US)\<close>
+  \<open>C \<in># dom_m N \<Longrightarrow> irred N C \<Longrightarrow> clss_size (fmdrop C N) NE UE NS US = (clss_size N NE UE NS US)\<close>
+  by (auto simp: clss_size_def ran_m_fmdrop_If clss_size_decr_lcount_def
+     size_remove1_mset_If clss_size_resetUS_def)
+
+
+lemma clss_size_lcount_clss_size[simp]:
+  \<open>clss_size_lcount (clss_size N NE UE NS US) = size (learned_clss_l N)\<close>
+  \<open>clss_size_allcount (clss_size N NE UE NS US) = size (learned_clss_l N) + size UE + size US\<close>
+  by (auto simp: clss_size_lcount_def clss_size_def clss_size_allcount_def)
+
+lemma clss_size_resetUS_simp[simp]:
+  \<open>clss_size_resetUS (clss_size_decr_lcount (clss_size baa da ea fa ga)) =
+     clss_size_decr_lcount (clss_size baa da ea fa {#})\<close>
+  \<open>clss_size_resetUS (clss_size_incr_lcount (clss_size baa da ea fa ga)) =
+     clss_size_incr_lcount (clss_size baa da ea fa {#})\<close>
+  \<open>clss_size_resetUS (clss_size_incr_lcountUE (clss_size baa da ea fa ga)) =
+     clss_size_incr_lcountUE (clss_size baa da ea fa {#})\<close>
+  \<open>clss_size_resetUS (clss_size N NE UE NS US) = (clss_size N NE UE NS {#})\<close>
+  by (auto simp: clss_size_resetUS_def clss_size_decr_lcount_def clss_size_def
+    clss_size_incr_lcount_def clss_size_incr_lcountUE_def)
+
+lemma [simp]: \<open>clss_size_resetUS (clss_size_incr_lcountUE st) =
+         clss_size_incr_lcountUE (clss_size_resetUS st)\<close>
+  by (solves \<open>cases st; auto simp: clss_size_incr_lcountUE_def clss_size_resetUS_def\<close>)+
+
+lemma clss_size_lcount_simps2[simp]:
+  \<open>clss_size_lcount (clss_size_resetUS S) = clss_size_lcount S\<close>
+  \<open>clss_size_lcountUE (clss_size_resetUS S) = clss_size_lcountUE S\<close>
+  \<open>clss_size_lcountUS (clss_size_resetUS S) = 0\<close>
+
+
+  \<open>clss_size_lcount (clss_size_incr_lcountUE S) = clss_size_lcount S\<close>
+  \<open>clss_size_lcountUE (clss_size_incr_lcountUE S) = Suc (clss_size_lcountUE S)\<close>
+  \<open>clss_size_lcountUS (clss_size_incr_lcountUE S) = clss_size_lcountUS S\<close>
+
+
+  \<open>clss_size_lcount (clss_size_decr_lcount S) = clss_size_lcount S - 1\<close>
+  \<open>clss_size_lcountUE (clss_size_decr_lcount S) = clss_size_lcountUE S\<close>
+  \<open>clss_size_lcountUS (clss_size_decr_lcount S) = clss_size_lcountUS S\<close>
+
+  \<open>clss_size_incr_lcountUE (clss_size_decr_lcount S) =
+        clss_size_decr_lcount (clss_size_incr_lcountUE S)\<close>
+  \<open>clss_size_resetUS (clss_size_decr_lcount S) = 
+     clss_size_decr_lcount (clss_size_resetUS S)\<close>
+  \<open>clss_size_resetUS (clss_size_incr_lcountUE S) = clss_size_incr_lcountUE (clss_size_resetUS S)\<close>
+  by (solves \<open>cases S; auto simp: clss_size_lcount_def clss_size_resetUS_def
+    clss_size_lcountUE_def clss_size_lcountUS_def
+    clss_size_incr_lcountUE_def clss_size_decr_lcount_def\<close>)+
+
+end
