Weidenbach_Book/IsaSAT/IsaSAT_Stats_LLVM.thy
@@ -1,0 +1,205 @@
+theory IsaSAT_Stats_LLVM
+imports IsaSAT_Stats IsaSAT_EMA_LLVM
+begin
+  abbreviation stats_rel :: \<open>(stats \<times> stats) set\<close> where
+  \<open>stats_rel \<equiv> word64_rel \<times>\<^sub>r word64_rel \<times>\<^sub>r word64_rel \<times>\<^sub>r word64_rel \<times>\<^sub>r word64_rel
+     \<times>\<^sub>r word64_rel \<times>\<^sub>r word64_rel \<times>\<^sub>r ema_rel\<close>
+
+abbreviation stats_assn :: \<open>stats \<Rightarrow> stats \<Rightarrow> assn\<close> where
+  \<open>stats_assn \<equiv> word64_assn \<times>\<^sub>a word64_assn \<times>\<^sub>a  word64_assn \<times>\<^sub>a word64_assn \<times>\<^sub>a word64_assn \<times>\<^sub>a
+     word64_assn \<times>\<^sub>a word64_assn \<times>\<^sub>a ema_assn\<close>
+
+
+lemma [sepref_import_param]:
+  \<open>(incr_propagation,incr_propagation) \<in> stats_rel \<rightarrow> stats_rel\<close>
+  \<open>(incr_conflict,incr_conflict) \<in> stats_rel \<rightarrow> stats_rel\<close>
+  \<open>(incr_decision,incr_decision) \<in> stats_rel \<rightarrow> stats_rel\<close>
+  \<open>(incr_restart,incr_restart) \<in> stats_rel \<rightarrow> stats_rel\<close>
+  \<open>(incr_lrestart,incr_lrestart) \<in> stats_rel \<rightarrow> stats_rel\<close>
+  \<open>(incr_uset,incr_uset) \<in> stats_rel \<rightarrow> stats_rel\<close>
+  \<open>(incr_GC,incr_GC) \<in> stats_rel \<rightarrow> stats_rel\<close>
+  \<open>(add_lbd,add_lbd) \<in> word32_rel \<rightarrow> stats_rel \<rightarrow> stats_rel\<close>
+  by auto
+
+lemmas [llvm_inline] =
+  incr_propagation_def
+  incr_conflict_def
+  incr_decision_def
+  incr_restart_def
+  incr_lrestart_def
+  incr_uset_def
+  incr_GC_def
+
+
+abbreviation (input) \<open>restart_info_rel \<equiv> word64_rel \<times>\<^sub>r word64_rel \<times>\<^sub>r word64_rel \<times>\<^sub>r word64_rel \<times>\<^sub>r word64_rel\<close>
+
+abbreviation (input) restart_info_assn where
+  \<open>restart_info_assn \<equiv> word64_assn \<times>\<^sub>a word64_assn \<times>\<^sub>a word64_assn \<times>\<^sub>a word64_assn \<times>\<^sub>a word64_assn\<close>
+
+lemma restart_info_params[sepref_import_param]:
+  "(incr_conflict_count_since_last_restart,incr_conflict_count_since_last_restart) \<in>
+    restart_info_rel \<rightarrow> restart_info_rel"
+  "(restart_info_update_lvl_avg,restart_info_update_lvl_avg) \<in>
+    word32_rel \<rightarrow> restart_info_rel \<rightarrow> restart_info_rel"
+  \<open>(restart_info_init,restart_info_init) \<in> restart_info_rel\<close>
+  \<open>(restart_info_restart_done,restart_info_restart_done) \<in> restart_info_rel \<rightarrow> restart_info_rel\<close>
+  by auto
+
+lemmas [llvm_inline] =
+  incr_conflict_count_since_last_restart_def
+  restart_info_update_lvl_avg_def
+  restart_info_init_def
+  restart_info_restart_done_def
+
+
+
+sepref_register NORMAL_PHASE QUIET_PHASE DEFAULT_INIT_PHASE
+
+sepref_def NORMAL_PHASE_impl
+  is \<open>uncurry0 (RETURN NORMAL_PHASE)\<close>
+  :: \<open>unit_assn\<^sup>k \<rightarrow>\<^sub>a word_assn\<close>
+  unfolding NORMAL_PHASE_def
+  by sepref
+
+sepref_def QUIET_PHASE_impl
+  is \<open>uncurry0 (RETURN QUIET_PHASE)\<close>
+  :: \<open>unit_assn\<^sup>k \<rightarrow>\<^sub>a word_assn\<close>
+  unfolding QUIET_PHASE_def
+  by sepref
+
+definition lcount_assn :: \<open>clss_size \<Rightarrow> _ \<Rightarrow> assn\<close> where
+  \<open>lcount_assn \<equiv> uint64_nat_assn \<times>\<^sub>a uint64_nat_assn \<times>\<^sub>a uint64_nat_assn\<close>
+
+lemma [safe_constraint_rules]:
+  \<open>CONSTRAINT Sepref_Basic.is_pure lcount_assn\<close>
+  unfolding lcount_assn_def
+  by auto
+
+sepref_def clss_size_lcount_fast_code
+  is \<open>RETURN o clss_size_lcount\<close>
+  :: \<open>lcount_assn\<^sup>k \<rightarrow>\<^sub>a uint64_nat_assn\<close>
+  unfolding clss_size_lcount_def lcount_assn_def
+  by sepref
+
+sepref_register clss_size_resetUS
+
+lemma clss_size_resetUS_alt_def:
+  \<open>RETURN o clss_size_resetUS =
+  (\<lambda>(lcount, lcountUE, lcountUS). RETURN (lcount, lcountUE, 0))\<close>
+  by (auto simp: clss_size_resetUS_def)
+
+sepref_def clss_size_resetUS_fast_code
+  is \<open>RETURN o clss_size_resetUS\<close>
+  :: \<open>lcount_assn\<^sup>d \<rightarrow>\<^sub>a lcount_assn\<close>
+  unfolding clss_size_resetUS_alt_def lcount_assn_def
+  apply (annot_unat_const \<open>TYPE(64)\<close>)
+  by sepref
+
+lemma clss_size_incr_lcountUS_alt_def:
+  \<open>RETURN o clss_size_incr_lcountUS =
+  (\<lambda>(lcount, lcountUE, lcountUS). RETURN (lcount, lcountUE, lcountUS + 1))\<close>
+  by (auto simp: clss_size_incr_lcountUS_def)
+
+sepref_def clss_size_incr_lcountUS_fast_code
+  is \<open>RETURN o clss_size_incr_lcountUS\<close>
+  :: \<open>[\<lambda>S. clss_size_lcountUS S < uint64_max]\<^sub>a lcount_assn\<^sup>d \<rightarrow> lcount_assn\<close>
+  unfolding clss_size_incr_lcountUS_alt_def lcount_assn_def clss_size_lcountUS_def
+  apply (annot_unat_const \<open>TYPE(64)\<close>)
+  by sepref
+
+lemma clss_size_incr_lcountUE_alt_def:
+  \<open>RETURN o clss_size_incr_lcountUE =
+  (\<lambda>(lcount, lcountUE, lcountUS). RETURN (lcount, lcountUE + 1, lcountUS))\<close>
+  by (auto simp: clss_size_incr_lcountUE_def)
+
+sepref_def clss_size_incr_lcountUE_fast_code
+  is \<open>RETURN o clss_size_incr_lcountUE\<close>
+  :: \<open>[\<lambda>S. clss_size_lcountUE S < uint64_max]\<^sub>a lcount_assn\<^sup>d \<rightarrow> lcount_assn\<close>
+  unfolding clss_size_incr_lcountUE_alt_def lcount_assn_def clss_size_lcountUE_def
+  apply (annot_unat_const \<open>TYPE(64)\<close>)
+  by sepref
+
+schematic_goal mk_free_lookup_clause_rel_assn[sepref_frame_free_rules]: \<open>MK_FREE lcount_assn ?fr\<close>
+  unfolding lcount_assn_def
+  by (rule free_thms sepref_frame_free_rules)+ (* TODO: Write a method for that! *)
+
+lemma clss_size_lcountUE_alt_def:
+  \<open>RETURN o clss_size_lcountUE = (\<lambda>(lcount, lcountUE, lcountUS). RETURN lcountUE)\<close>
+  by (auto simp: clss_size_lcountUE_def)
+
+sepref_def clss_size_lcountUE_fast_code
+  is \<open>RETURN o clss_size_lcountUE\<close>
+  :: \<open>lcount_assn\<^sup>k \<rightarrow>\<^sub>a uint64_nat_assn\<close>
+  unfolding lcount_assn_def clss_size_lcountUE_alt_def clss_size_lcount_def
+  by sepref
+
+lemma clss_size_lcountUS_alt_def:
+  \<open>RETURN o clss_size_lcountUS = (\<lambda>(lcount, lcountUE, lcountUS). RETURN lcountUS)\<close>
+  by (auto simp: clss_size_lcountUS_def)
+
+sepref_def clss_size_lcountUSt_fast_code
+  is \<open>RETURN o clss_size_lcountUS\<close>
+  :: \<open>lcount_assn\<^sup>k \<rightarrow>\<^sub>a uint64_nat_assn\<close>
+  unfolding lcount_assn_def clss_size_lcountUS_alt_def clss_size_lcount_def
+  by sepref
+
+lemma clss_size_incr_allcount_alt_def:
+  \<open>RETURN o clss_size_allcount =
+  (\<lambda>(lcount, lcountUE, lcountUS). RETURN (lcount + lcountUE + lcountUS))\<close>
+  by (auto simp: clss_size_allcount_def)
+
+sepref_def clss_size_allcount_fast_code
+  is \<open>RETURN o clss_size_allcount\<close>
+  :: \<open>[\<lambda>S. clss_size_allcount S < max_snat 64]\<^sub>a lcount_assn\<^sup>d \<rightarrow> uint64_nat_assn\<close>
+  unfolding clss_size_incr_allcount_alt_def lcount_assn_def clss_size_allcount_def
+  by sepref
+
+
+lemma clss_size_decr_lcount_alt_def:
+  \<open>RETURN o clss_size_decr_lcount =
+  (\<lambda>(lcount, lcountUE, lcountUS). RETURN (lcount - 1, lcountUE, lcountUS))\<close>
+  by (auto simp: clss_size_decr_lcount_def)
+
+sepref_def clss_size_decr_lcount_fast_code
+  is \<open>RETURN o clss_size_decr_lcount\<close>
+  :: \<open>[\<lambda>S. clss_size_lcount S \<ge> 1]\<^sub>a lcount_assn\<^sup>d \<rightarrow> lcount_assn\<close>
+  unfolding lcount_assn_def clss_size_decr_lcount_alt_def clss_size_lcount_def
+  apply (annot_unat_const \<open>TYPE(64)\<close>)
+  by sepref
+
+
+lemma emag_get_value_alt_def:
+  \<open>ema_get_value = (\<lambda>(a, b, c, d). a)\<close>
+  by auto
+
+sepref_def ema_get_value_impl
+  is \<open>RETURN o ema_get_value\<close>
+  :: \<open>ema_assn\<^sup>k \<rightarrow>\<^sub>a word_assn\<close>
+  unfolding emag_get_value_alt_def
+  by sepref
+
+definition ema_extract_value_coeff :: \<open>nat\<close> where
+  [simp]: \<open>ema_extract_value_coeff = 32\<close>
+
+sepref_register ema_extract_value_coeff
+
+lemma ema_extract_value_32[sepref_fr_rules]:
+  \<open>(uncurry0 (return (32 :: 64 word)), uncurry0 (RETURN ema_extract_value_coeff)) \<in> unit_assn\<^sup>k \<rightarrow>\<^sub>a unat_assn\<close>
+  apply sepref_to_hoare
+  apply vcg
+  apply (auto simp: ENTAILS_def unat_rel_def unat.rel_def br_def pred_lift_merge_simps)
+  by (metis (mono_tags, lifting) entails_def entails_lift_extract_simps(2) frame_thms(2))
+
+lemmas [llvm_inline] = ema_extract_value_coeff_def
+
+lemma emag_extract_value_alt_def:
+  \<open>ema_extract_value = (\<lambda>(a, b, c, d). a >> ema_extract_value_coeff)\<close>
+  by auto
+
+sepref_def ema_extract_value_impl
+  is \<open>RETURN o ema_extract_value\<close>
+  :: \<open>ema_assn\<^sup>k \<rightarrow>\<^sub>a word_assn\<close>
+  unfolding emag_extract_value_alt_def ema_extract_value_coeff_def[symmetric]
+  by sepref
+
+end
